sketch view morphisms

src/Iris/Algebra/View.lean
@@ -644,4 +644,62 @@ theorem auth_alloc (Hup : ∀ n bf, R n a bf → R n a (b • bf)) :
 -- TODO: Local update lemma
 
 end Updates
+
+section ViewMap
+
+/- [OFE A] [UCMRA B] [OFE A'] [UCMRA B'] -/
+
+def View.map  {R : ViewRel A B} (R' : ViewRel A' B') (f : A → A') (g : B → B') (v : View F R) : View F R' where
+  auth := match v.auth with
+    | none => none
+    | some (fr, a) => (fr, a.map' f)
+  frag := g v.frag
+
+theorem View.map_id {R : ViewRel A B} (v : View F R) :
+    View.map R id id v = v := by
+  simp [View.map, Agree.map']
+  rcases v with ⟨a, b⟩
+  cases a <;> simp
+
+theorem View.map_compose {R : ViewRel A B} {R' : ViewRel A' B'} {R'' : ViewRel A'' B''} f g (f' : A' → A'') (g' : B' → B'') (v : View F R) :
+    View.map R'' (f' ∘ f) (g' ∘ g) v = View.map R'' f' g' (View.map R' f g v) := by
+  simp [View.map, Agree.map']
+  rcases v with ⟨a, b⟩
+  cases a <;> simp
+
+theorem View.map_ext [OFE A] [OFE B] [OFE A'] [OFE B'] {R : ViewRel A B} {R' : ViewRel A' B'} (f1 f2 : A → A') (g1 g2 : B → B') [OFE.NonExpansive f1] [OFE.NonExpansive f2] (v : View F R) :
+    (∀ a, f1 a ≡ f2 a) → (∀ b, g1 b ≡ g2 b) →
+    View.map R' f1 g1 v ≡ View.map R' f2 g2 v := by
+  intro h1 h2
+  simp [View.map]
+  constructor <;> simp only
+  · split <;> constructor <;> simp
+    apply Agree.agree_map_ext h1
+  · apply h2
+
+instance View.map_ne [OFE A] [OFE B] [OFE A'] [OFE B'] {R : ViewRel A B} {R' : ViewRel A' B'} (f : A → A') (g : B → B') [OFE.NonExpansive f] [hne : OFE.NonExpansive g] : OFE.NonExpansive (View.map R' f g : (View F R → _)) where
+  ne := by
+    rintro n ⟨a1, b1⟩ ⟨a2, b2⟩ ⟨h1, h2⟩
+    constructor <;> simp [map]
+    · split <;> split <;> simp_all
+      cases h1
+      constructor <;> simp_all
+      apply (Agree.map f).ne.ne
+      simp_all only
+    · apply hne.ne
+      simp_all only [instCOFEDFrac]
+
+instance View.mapO [OFE A] [OFE B] [OFE A'] [OFE B'] {R : ViewRel A B} {R' : ViewRel A' B'} (f : A -n> A') (g : B -n> B') : View F R -n> View F R' where
+  f := View.map R' f g
+  ne := inferInstance
+
+instance View.mapC [UFraction F] [OFE A] [UCMRA B] [OFE A'] [UCMRA B'] {R : ViewRel A B} [IsViewRel R] {R' : ViewRel A' B'} [IsViewRel R'] (f : A -n> A') (g : B -C> B') (H : ∀ n a b, R n a b → R' n (f a) (g b)) : View F R -C> View F R' where
+  f := View.map R' f g
+  ne := inferInstance
+  validN := sorry
+  pcore := sorry
+  op := sorry
+
+end ViewMap
+
 end View
